Prove result about bijections and "simple loops" over primitives w/failure

hol/monadicPrimitivesScript.sml
@@ -3,7 +3,6 @@ open HolKernel Parse boolLib bossLib;
 open lcsymtacs
 open pred_setTheory
 open monadsyntax
-open forLoopTheory
 
 val _ = new_theory "monadicPrimitives";
 
@@ -12,19 +11,26 @@ val _ = overload_on ("monad_bind", ``OPTION_BIND``)
 val _ = overload_on ("monad_unitbind", ``OPTION_IGNORE_BIND``)
 val _ = ParseExtras.tight_equality()
 
-val _ = type_abbrev ("mvector", ``:(num -> 'a) # num``)
+val _ = type_abbrev ("mvector", ``:'a list``)
+val _ = disable_tyabbrev_printing "mvector"
 val SAT_ss = SatisfySimps.SATISFY_ss
 val _ = augment_srw_ss [SAT_ss]
 
+fun csimp thl = asm_simp_tac (srw_ss() ++ boolSimps.CONJ_ss) thl
+fun asimp thl = asm_simp_tac (srw_ss() ++ ARITH_ss) thl
+fun acsimp thl = asm_simp_tac (srw_ss() ++ boolSimps.CONJ_ss ++ ARITH_ss) thl
+val bsimp = asm_simp_tac bool_ss
+
 val vsub_def = Define`
-  vsub (mv, sz) i = if i < sz then SOME (mv i) else NONE
+  vsub l i = if i < LENGTH l then SOME (EL i l) else NONE
 `
 
 val _ = set_fixity "'" (Infixl 2000)
 val _ = overload_on ("'", ``vsub``)
-val _ = overload_on ("vsz", ``SND : (num -> 'a) # num -> num``)
+val _ = overload_on ("vsz", ``LENGTH : 'a list -> num``)
+val _ = overload_on ("LENGTH", listSyntax.length_tm)
 
-val empty_v_def = Define`empty_v n v = (K v, n)`
+val empty_v_def = Define`empty_v n v = GENLIST (K v) n`
 
 val vsz_empty_v = store_thm(
   "vsz_empty_v",
@@ -46,12 +52,161 @@ val IGNORE_BIND_ASSOC = store_thm(
 val _ = export_rewrites ["IGNORE_BIND_ASSOC"]
 
 val update_def = Define`
-  update (mv,sz) d r = if d < sz then SOME ((d =+ r) mv, sz) else NONE
+  update l d r = if d < LENGTH l then SOME (LUPDATE r d l) else NONE
 `;
 
-val mvector_to_list_def = Define`
-  mvector_to_list (f,sz) = REVERSE (FOR (0,sz) (λi l. f i :: l) [])
-`;
+val EL_mvector_to_list = store_thm(
+  "EL_mvector_to_list",
+  ``i < vsz v ⇒ v ' i = SOME (EL i v)``,
+  simp[vsub_def]);
 
+val vector_EQ = store_thm(
+  "vector_EQ",
+  ``v1 : 'a mvector = v2 ⇔ (∀i. v1 ' i = v2 ' i) ∧ vsz v1 = vsz v2``,
+  simp[listTheory.LIST_EQ_REWRITE, vsub_def, EQ_IMP_THM] >>
+  metis_tac[TypeBase.one_one_of ``:'a option``]);
+
+val mFOR_def = tDefine "mFOR" `
+  mFOR (lo,hi) f A =
+    if lo < hi then
+      case f lo A of
+          NONE => NONE
+        | SOME A' => mFOR (lo+1,hi) f A'
+    else SOME A
+` (WF_REL_TAC `measure (λ((lo,hi),f,A). hi - lo)`)
+
+val mFOR_0 = store_thm(
+  "mFOR_0",
+  ``mFOR (x,x) f A = SOME A``,
+  simp[Once mFOR_def]);
+val _ = export_rewrites ["mFOR_0"]
+
+val mFOR_thm = store_thm(
+  "mFOR_thm",
+  ``(hi ≤ lo ⇒ mFOR (lo,hi) f A = SOME A) ∧
+    (lo < hi ⇒ mFOR (lo,hi) f A =
+               do
+                 A' <- f lo A;
+                 mFOR (lo+1,hi) f A'
+               od)``,
+  strip_tac >> simp[Once mFOR_def, SimpLHS] >>
+  Cases_on `f lo A` >> simp[]);
+
+val mFOR_RULE = store_thm(
+  "mFOR_RULE",
+  ``∀lo hi f A P Inv.
+      Inv lo A ∧
+      (∀i s0. lo ≤ i ∧ i < hi ∧ Inv i s0 ⇒ ∃s. f i s0 = SOME s ∧ Inv (i + 1) s) ∧
+      (∀i s. hi ≤ i ⇒ Inv i s ⇒ P (SOME s)) ⇒
+      P (mFOR (lo,hi) f A)``,
+  rpt gen_tac >>
+  qid_spec_tac `A` >> Induct_on `hi - lo`
+  >- srw_tac[ARITH_ss][mFOR_thm] >>
+  srw_tac[][] >>
+  `lo ≤ lo ∧ lo < hi` by decide_tac >>
+  `∃A'. f lo A = SOME A' ∧ Inv (lo + 1) A'` by metis_tac[] >>
+  srw_tac[ARITH_ss][mFOR_thm]);
+
+val _ = overload_on ("''", ``λa i. OPTION_BIND a (combin$C vsub i)``)
+val _ = set_fixity "''" (Infixl 2000)
+
+val vsub_assert = store_thm(
+  "vsub_assert",
+  ``A ' i = do assert(i < vsz A); SOME (EL i A) od``,
+  rw[vsub_def]);
+
+val update_assert = store_thm(
+  "update_assert",
+  ``update A i v = do assert(i < vsz A); SOME(LUPDATE v i A) od``,
+  rw[update_def]);
+
+val mFOR_CONG = store_thm(
+  "mFOR_CONG",
+  ``(∀j A. j < hi ⇒ (f j A = f' j A)) ⇒
+    mFOR (lo,hi) f A = mFOR (lo,hi) f' A``,
+  strip_tac >> qid_spec_tac `A` >>
+  Induct_on `hi - lo` >> asm_simp_tac(srw_ss() ++ ARITH_ss) [mFOR_thm]);
+
+val PERMS_suffice0 = prove(
+  ``BIJ (THE o vsub Δ) (count N) (count N) ∧ vsz Δ = N ∧ N ≤ vsz A1 ∧
+    SOME final = mFOR (0, N) (λi A. update A i (g i)) A1 ⇒
+    ∀m n A2:α list.
+      vsz A2 = vsz A1 ∧
+      (m = N - n) ∧ n ≤ N ∧
+      (∀i. i < vsz A2 ⇒
+           A2 ' i = if i ∈ IMAGE (THE o vsub Δ) (count n) then final ' i
+                    else A1 ' i)
+   ⇒
+      mFOR (n,N) (λj A. do i <- Δ ' j ; update A i (g i) od) A2 = SOME final``,
+  strip_tac >>
+  `vsz final = vsz A1 ∧
+   ∀i. i < vsz A1 ⇒ EL i final = if i < N then g i else EL i A1`
+    by (qpat_assum `SOME final = XX` mp_tac >>
+        DEEP_INTRO_TAC mFOR_RULE >>
+        qexists_tac
+          `λi A. vsz A = vsz A1 ∧
+                 ∀j. j < vsz A1 ⇒ EL j A = if j < i ∧ j < N then g j
+                                           else EL j A1` >>
+        srw_tac[ARITH_ss][update_assert, listTheory.EL_LUPDATE] >>
+        srw_tac[][] >> full_simp_tac(srw_ss() ++ ARITH_ss) []) >>
+  `∀i. i < N ⇒ EL i Δ < N`
+    by (qpat_assum `BIJ ff ss tt` mp_tac >>
+        simp[BIJ_IFF_INV, vsub_def]) >>
+  Induct >| [
+    rpt strip_tac >> `N = n` by decide_tac >> qpat_assum `0 = N - n` kall_tac >>
+    srw_tac[ARITH_ss][] >>
+    `A2 = final` suffices_by simp[] >>
+    srw_tac[ARITH_ss][listTheory.LIST_EQ_REWRITE] >>
+    Cases_on `x < LENGTH Δ`
+    >- (`x ∈ IMAGE (THE o $' Δ) (count (LENGTH Δ))`
+           by (simp[] >> qpat_assum `BIJ ff ss tt` mp_tac >>
+               simp[BIJ_IFF_INV, vsub_def] >>
+               asm_simp_tac(srw_ss() ++ boolSimps.CONJ_ss) [] >>
+               metis_tac[]) >>
+        first_x_assum (qspec_then `x` mp_tac) >>
+        asm_simp_tac bool_ss [] >>
+        simp[vsub_def]) >>
+    first_x_assum (qspec_then `x` mp_tac) >>
+    asm_simp_tac(srw_ss() ++ ARITH_ss)[vsub_def],
+
+    rpt strip_tac >>
+    asm_simp_tac(srw_ss() ++ ARITH_ss) [mFOR_thm, SimpLHS] >>
+    `Δ ' n = do assert (n < vsz Δ); SOME(EL n Δ) od` by simp[vsub_assert] >>
+    FREEZE_THEN
+      (fn th => REWRITE_TAC [th])
+      (update_assert |> Q.GEN `i` |> Q.GEN `v` |> Q.INST [`A` |-> `A2`]) >>
+    `n < N` by decide_tac >>
+    `EL n Δ < LENGTH A1` by metis_tac[DECIDE ``x < y ∧ y ≤ z ⇒ x < z``] >>
+    asm_simp_tac (srw_ss() ++ ARITH_ss) [] >>
+    qpat_assum `SOME final = XX` (ASSUME_TAC o SYM) >> simp[] >>
+    first_x_assum match_mp_tac >> simp[] >> rpt strip_tac >>
+    asm_simp_tac(srw_ss() ++ ARITH_ss ++ boolSimps.CONJ_ss)[vsub_assert] >>
+    Cases_on `i = EL n Δ` >> simp[]
+    >- (reverse (rw[]) >- metis_tac[DECIDE ``n < n + 1``] >>
+        simp[listTheory.EL_LUPDATE]) >>
+    Cases_on `∃j. i = EL j Δ ∧ j < n + 1`
+    >- (simp[] >> pop_assum strip_assume_tac >>
+        `j < n` by metis_tac[DECIDE ``x < y + 1 ⇔ x < y ∨ x = y``] >> simp[] >>
+        `i ∈ IMAGE (THE o $' Δ) (count n)`
+          by (simp[vsub_assert] >> acsimp[] >> metis_tac[]) >>
+        first_x_assum (qspec_then `i` mp_tac) >>
+        asm_simp_tac bool_ss [] >>
+        simp[vsub_def, listTheory.EL_LUPDATE]) >>
+    simp[] >>
+    `i ∉ IMAGE (THE o $' Δ) (count n)`
+      by (simp[vsub_def] >> qx_gen_tac `j` >> Cases_on `j < n` >> simp[] >>
+          metis_tac[DECIDE ``j < n ⇒ j < n + 1``]) >>
+    first_x_assum (qspec_then `i` mp_tac) >> bsimp[] >>
+    simp[vsub_def, listTheory.EL_LUPDATE]
+  ]);
+
+val PERMS_SUFFICE_simple = save_thm(
+  "PERMS_SUFFICE_simple",
+  PERMS_suffice0 |> SIMP_RULE (srw_ss()) []
+                 |> UNDISCH
+                 |> Q.SPECL [`0`, `A1`]
+                 |> SIMP_RULE (srw_ss()) []
+                 |> DISCH_ALL
+                 |> Q.INST [`A1` |-> `A`]);
 
 val _ = export_theory();
